prove the parts of ceval'_derive irrelavent to arbitary_eval, some hole remains

ASTLc_woc.v
@@ -199,7 +199,7 @@ Inductive ceval' : func_context -> com -> label -> label -> state -> state -> Pr
       valid_label l2 ->
       ceval' fc c l1 (com_to_label_pure c) st1 st3 ->
       ceval' fc (CWhile b c) (LWhile b (com_to_label_pure c)) l2 st3 st2 ->
-      ceval' fc (CWhile b c) l1 l2 st1 st2
+      ceval' fc (CWhile b c) (LWhile b l1) l2 st1 st2
 
   | E'_Reentry1c : forall fc st,
       ceval' fc CReentry LPure LHere st st
@@ -266,7 +266,7 @@ Proof.
     assumption.
   - split; right; apply SP_While; assumption.
   - split.
-    right; assumption.
+    right; apply SP_While; assumption.
     assumption.
   - split.
     left; apply IP_Pure.
@@ -289,6 +289,10 @@ Inductive middle_ceval' : func_context -> public_funcs -> restk -> restk -> Prop
       single_point l2 ->
       ceval' fc c l1 l2 st1 st2 ->
       middle_ceval' fc lf ((c, Some l1, st1) :: stk) ((c, Some l2, st2) :: stk)
+(*   | ME_r_while : forall fc lf b c l1 st1 st2 stk,
+      ceval' fc (CWhile b c) l1 (com_to_label_pure (CWhile b c)) st1 st2 ->
+      middle_ceval' fc lf (((CWhile b c), Some l1, st1) :: stk)
+        (((CWhile b c), Some (com_to_label_pure (CWhile b c)), st2) :: stk) *)
   | ME_re : forall fc c1 c2 l1 loc1 loc2 glb stk lf f,
       In f lf ->
       c2 = snd (fc f) ->
@@ -895,6 +899,395 @@ Unshelve.
 Qed.
 (** Seq Tail *)
 
+(** If Branch *)
+Lemma middle_ceval'_if_branch_some:
+  forall fc lf b c1 c2 l1 l2 stk1 stk2 st1 st2,
+  single_point l1 ->
+  middle_ceval' fc lf
+    (stk1 ++ (c1, Some l1, st1) :: nil)
+    (stk2 ++ (c1, Some l2, st2) :: nil) ->
+  middle_ceval' fc lf
+    (stk1 ++ (CIf b c1 c2, Some (LIf b l1 (com_to_label_pure c2)), st1) :: nil)
+    (stk2 ++ (CIf b c1 c2, Some (LIf b l2 (com_to_label_pure c2)), st2) :: nil).
+Proof.
+  intros.
+  destruct stk1, stk2; simpl in *.
+  - inversion H0; subst.
+    eapply E'_If1, ME_r_single in H10.
+    exact H10.
+    apply SP_If1.
+    exact H5.
+    apply com_to_label_pure_is_pure.
+    exact H.
+    right. exact H5.
+  - inversion H0; subst.
+    + pose proof eq_refl (@length (com * option label * state) nil).
+      rewrite H9 in H1 at 1.
+      rewrite app_length in H1.
+      simpl in H1. omega.
+    + pose proof eq_refl (@length (com * option label * state) nil).
+      rewrite H9 in H1 at 1.
+      rewrite app_length in H1.
+      simpl in H1. omega.
+    + destruct stk2; simpl in *.
+      2:{
+        pose proof (eq_refl (length ((c1, Some l1, (loc1, glb)) :: nil))).
+        rewrite H9 in H1 at 1.
+        simpl in H1.
+        rewrite app_length in H1.
+        simpl in H1. omega.
+      }
+      inversion H9; subst; clear H9.
+      eapply ME_re.
+      exact H6.
+      auto.
+      apply SP_If1.
+      exact H11. apply com_to_label_pure_is_pure.
+  - inversion H0; subst.
+    + pose proof eq_refl (@length (com * option label * state) nil).
+      rewrite <- H9 in H1 at 1.
+      rewrite app_length in H1.
+      simpl in H1. omega.
+    + destruct stk1; simpl in *.
+      2:{
+        pose proof (eq_refl (length ((c1, Some l2, (loc2, glb2)) :: nil))).
+        rewrite H5 in H1 at 1.
+        simpl in H1.
+        rewrite app_length in H1.
+        simpl in H1. omega.
+      }
+      inversion H5; subst.
+      eapply ME_ex.
+      apply SP_If1.
+      exact H4. apply com_to_label_pure_is_pure.
+  - inversion H0; subst.
+    + apply app_inj_tail in H7 as [? ?];
+      inversion H2; subst; clear H2.
+      eapply ME_r_pure in H4.
+      exact H4.
+    + apply app_inj_tail in H7 as [? ?];
+      inversion H2; subst; clear H2.
+      eapply ME_r_single in H8.
+      exact H8. exact H6.
+    + rewrite app_comm_cons in H6.
+      apply app_inj_tail in H6 as [? ?];
+      inversion H2; subst; clear H2.
+      eapply ME_re.
+      exact H7.
+      auto.
+      exact H9.
+    + rewrite app_comm_cons in H5.
+      apply app_inj_tail in H5 as [? ?];
+      inversion H2; subst; clear H2.
+      eapply ME_ex.
+      exact H4.
+Qed.
+
+Lemma multi_ceval'_if_branch:
+  forall fc lf b c1 c2 l1 st3 st2,
+  single_point l1 ->
+  clos_trans restk (middle_ceval' fc lf)
+    ((c1, Some l1, st3) :: nil)
+    ((c1, None, st2) :: nil) ->
+  clos_trans restk (middle_ceval' fc lf)
+    ((CIf b c1 c2, Some (LIf b l1 (com_to_label_pure c2)), st3) :: nil)
+    ((CIf b c1 c2, None, st2) :: nil).
+Proof.
+  intros.
+  apply Operators_Properties.clos_trans_t1n in H0.
+  set (stk := @nil (com * option label * state)).
+  unfold stk.
+  change ((c1, Some l1, st3) :: nil) with (stk ++ (c1, Some l1, st3) :: nil) in H0.
+  change ((CIf b c1 c2, Some (LIf b l1 (com_to_label_pure c2)), st3) :: nil) with (stk ++ (CIf b c1 c2, Some (LIf b l1 (com_to_label_pure c2)), st3) :: nil).
+  clearbody stk.
+  remember (stk ++ (c1, Some l1, st3) :: nil) as stk1.
+  remember ((c1, None, st2) :: nil) as stk2.
+  generalize dependent stk.
+  revert st3.
+  generalize dependent l1.
+  induction H0; intros; subst.
+  - destruct stk; simpl in *; inversion H; subst.
+    + eapply E'_If1, ME_r_pure, t_step in H4; try assumption.
+      exact H4. apply com_to_label_pure_valid.
+    + pose proof eq_refl (length (stk ++ (c1, Some l1, st3) :: nil)).
+      rewrite H8 in H1 at 1.
+      rewrite app_length in H1.
+      simpl in H1. omega.
+  - specialize (IHclos_trans_1n (eq_refl _)).
+    inversion H; subst.
+    + destruct stk; simpl in *; inversion H2; subst; clear H2.
+      * inversion H0; inversion H2.
+      * pose proof IHclos_trans_1n l1 H1 st3 ((c, None, st0) :: stk) (eq_refl _).
+        repeat rewrite app_comm_cons in H.
+        eapply middle_ceval'_if_branch_some, t_step in H.
+        eapply t_trans.
+        exact H. exact H2. exact H1.
+    + destruct stk; simpl in *; inversion H2; subst; clear H2.
+      * pose proof IHclos_trans_1n l2 H3 st0 nil (eq_refl _).
+        rewrite <- app_nil_l in H.
+        rewrite <- (@app_nil_l (com * option label * state)) in H at 1.
+        eapply middle_ceval'_if_branch_some, t_step in H.
+        simpl in *.
+        eapply t_trans.
+        exact H. exact H2. exact H1.
+      * pose proof IHclos_trans_1n l1 H1 st3 ((c, Some l2, st0) :: stk) (eq_refl _).
+        repeat rewrite app_comm_cons in H.
+        eapply middle_ceval'_if_branch_some, t_step in H.
+        eapply t_trans.
+        exact H. exact H2. exact H1.
+    + destruct stk; simpl in *; inversion H2; subst; clear H2.
+      * pose proof IHclos_trans_1n l1 H1 (loc1, glb) ((snd (fc f), Some (com_to_label_pure (snd (fc f))), (loc2, glb)) :: nil) (eq_refl _).
+        rewrite <- (@app_nil_l (_ * _ * _)) in H at 1.
+        rewrite (@cons_insert_nil (_ * _ * (_ * _))), app_comm_cons in H.
+        eapply middle_ceval'_if_branch_some, t_step in H.
+        simpl in *.
+        eapply t_trans.
+        exact H. exact H2. exact H1.
+      * pose proof IHclos_trans_1n l1 H1 st3 ((snd (fc f), Some (com_to_label_pure (snd (fc f))), (loc2, glb)) :: (c0, Some l0, (loc1, glb)) :: stk) (eq_refl _).
+        repeat rewrite app_comm_cons in H.
+        eapply middle_ceval'_if_branch_some, t_step in H.
+        simpl in *.
+        eapply t_trans.
+        exact H. exact H2. exact H1.
+    + destruct stk; simpl in *; inversion H2; subst; clear H2.
+      destruct stk; simpl in *; inversion H6; subst; clear H6.
+      * pose proof IHclos_trans_1n l1 H1 (loc2, glb1) nil (eq_refl _).
+        rewrite cons_insert_nil, app_comm_cons in H.
+        rewrite <- app_nil_l in H.
+        eapply middle_ceval'_if_branch_some, t_step in H.
+        simpl in *.
+        eapply t_trans.
+        exact H. exact H2. exact H1.
+      * pose proof IHclos_trans_1n l1 H1 st3 ((c3, Some l2, (loc2, glb1)) :: stk) (eq_refl _).
+        repeat rewrite app_comm_cons in H.
+        eapply middle_ceval'_if_branch_some, t_step in H.
+        eapply t_trans; [apply H | apply H2].
+        exact H1.
+Qed.
+(** If Branch *)
+
+(** Else Branch *)
+Lemma middle_ceval'_else_branch_some:
+  forall fc lf b c1 c2 l1 l2 stk1 stk2 st1 st2,
+  single_point l1 ->
+  middle_ceval' fc lf
+    (stk1 ++ (c2, Some l1, st1) :: nil)
+    (stk2 ++ (c2, Some l2, st2) :: nil) ->
+  middle_ceval' fc lf
+    (stk1 ++ (CIf b c1 c2, Some (LIf b (com_to_label_pure c2) l1), st1) :: nil)
+    (stk2 ++ (CIf b c1 c2, Some (LIf b (com_to_label_pure c2) l2), st2) :: nil).
+Proof.
+Admitted.
+
+Lemma multi_ceval'_else_branch:
+  forall fc lf b c1 c2 l1 st3 st2,
+  single_point l1 ->
+  clos_trans restk (middle_ceval' fc lf)
+    ((c2, Some l1, st3) :: nil)
+    ((c2, None, st2) :: nil) ->
+  clos_trans restk (middle_ceval' fc lf)
+    ((CIf b c1 c2, Some (LIf b (com_to_label_pure c1) l1), st3) :: nil)
+    ((CIf b c1 c2, None, st2) :: nil).
+Proof.
+Admitted.
+(** Else Branch *)
+
+(** While Loop *)
+Lemma middle_ceval'_while_loop:
+  forall fc lf b c l0 l1 st1 st2 stk1 stk2,
+  single_point l0 ->
+  middle_ceval' fc lf
+    (stk1 ++ (c, Some l0, st1) :: nil)
+    (stk2 ++ (c, Some l1, st2) :: nil) ->
+  middle_ceval' fc lf
+    (stk1 ++ (CWhile b c, Some (LWhile b l0), st1) :: nil)
+    (stk2 ++ (CWhile b c, Some (LWhile b l1), st2) :: nil).
+Proof.
+  intros.
+  destruct stk1, stk2; simpl in *.
+  - inversion H0; subst.
+    eapply E'_WhileSeg1 in H10; try assumption.
+    eapply ME_r_single in H10.
+    exact H10.
+    apply SP_While; assumption.
+  - inversion H0; subst.
+    + pose proof eq_refl (length (stk2 ++ (c, Some l1, st2) :: nil)).
+      rewrite <- H9 in H1 at 1.
+      rewrite app_length in H1.
+      simpl in H1. omega.
+    + pose proof eq_refl (length (stk2 ++ (c, Some l1, st2) :: nil)).
+      rewrite <- H9 in H1 at 1.
+      rewrite app_length in H1.
+      simpl in H1. omega.
+    + destruct stk2; simpl in *; inversion H9; subst.
+      * eapply ME_re.
+        exact H6.
+        auto.
+        apply SP_While, H11.
+      * pose proof eq_refl (length (stk2 ++ (c, Some l1, st2) :: nil)).
+        rewrite <- H3 in H1 at 1.
+        rewrite app_length in H1.
+        simpl in H1. omega.
+  - inversion H0; subst.
+    + pose proof increase_one_side (c, Some l0, st1) nil stk1.
+      congruence.
+    + destruct stk1; simpl in *; inversion H5; subst.
+      eapply ME_ex.
+      apply SP_While, H4.
+      pose proof increase_one_side (c, Some l0, st1) nil stk1.
+      symmetry in H3.
+      unfold state in H3.
+      congruence.
+  - inversion H0; subst.
+    + apply app_inj_tail in H7 as [? ?]; inversion H2; subst; clear H2.
+      eapply ME_r_pure in H4.
+      exact H4.
+    + apply app_inj_tail in H7 as [? ?]; inversion H2; subst; clear H2.
+      eapply ME_r_single in H8.
+      exact H8. exact H6.
+    + destruct stk2; simpl in *; inversion H6; subst.
+      * pose proof increase_one_side (c, Some l0, st1) nil stk1.
+        unfold state in H5.
+        congruence.
+      * apply app_inj_tail in H3 as [? ?]; inversion H2; subst; clear H6 H2.
+        eapply ME_re.
+        exact H7. auto. exact H9.
+    + destruct stk1; simpl in *; inversion H5; subst.
+      * pose proof increase_one_side (c, Some l1, st2) nil stk2.
+        unfold state in H7.
+        congruence.
+      * apply app_inj_tail in H3 as [? ?]; inversion H2; subst; clear H5 H2.
+        eapply ME_ex.
+        exact H4.
+Qed.
+
+Lemma multi_ceval'_while_loop:
+  forall fc lf b c l1 st1 st2,
+  beval st1 b = true ->
+  clos_trans restk (middle_ceval' fc lf)
+    ((c, Some (com_to_label_pure c), st1) :: nil)
+    ((c, Some l1, st2) :: nil) ->
+  clos_trans restk (middle_ceval' fc lf)
+    ((CWhile b c, Some (LWhile b (com_to_label_pure c)), st1) :: nil)
+    ((CWhile b c, Some (LWhile b l1), st2) :: nil).
+Proof.
+  intros.
+  apply Operators_Properties.clos_trans_tn1 in H0.
+  assert (single_point l1).
+  { inversion H0; inversion H1; assumption. }
+  set (stk := @nil (com * option label * state)).
+  unfold stk.
+  change ((c, Some l1, st2) :: nil) with (stk ++ (c, Some l1, st2) :: nil) in H0.
+  change ((CWhile b c, Some (LWhile b l1), st2) :: nil) with (stk ++ (CWhile b c, Some (LWhile b l1), st2) :: nil).
+  clearbody stk.
+  remember ((c, Some (com_to_label_pure c), st1) :: nil) as stk1.
+  remember (stk ++ (c, Some l1, st2) :: nil) as stk2.
+  generalize dependent stk.
+  revert st2.
+  generalize dependent l1.
+  induction H0; intros; subst.
+  - destruct stk; simpl in *; inversion H0; subst.
+    + eapply E'_WhileTrue1, ME_r_single, t_step in H11.
+      exact H11.
+      apply SP_While, H1.
+      apply com_to_label_pure_is_pure.
+      assumption.
+      assumption.
+    + pose proof eq_refl (length (stk ++ (c, Some l1, st2) :: nil)).
+      rewrite <- H10 in H2 at 1.
+      rewrite app_length in H2.
+      simpl in H2. omega.
+    + pose proof eq_refl (length (stk ++ (c, Some l1, st2) :: nil)).
+      rewrite <- H10 in H2 at 1.
+      rewrite app_length in H2.
+      simpl in H2. omega.
+    + pose proof com_to_label_pure_no_point c.
+      congruence.
+  - inversion H0; subst.
+    + destruct stk; simpl in *; inversion H3; subst; clear H3.
+      pose proof IHclos_trans_n1 l1 H2 st2 ((c0, Some l0, st0) :: stk) (eq_refl _).
+      repeat rewrite app_comm_cons in H0.
+      eapply middle_ceval'_while_loop, t_step in H0.
+      eapply t_trans.
+      exact H3. exact H0. exact H2.
+    + destruct stk; simpl in *; inversion H3; subst; clear H3.
+      * assert (single_point l0). { inversion H1; inversion H3; assumption. }
+        pose proof IHclos_trans_n1 l0 H3 st0 nil (eq_refl _).
+        rewrite <- app_nil_l in H0.
+        rewrite <- (@app_nil_l (_ * _ * _)) in H0 at 1.
+        eapply middle_ceval'_while_loop, t_step in H0.
+        simpl in *.
+        eapply t_trans.
+        exact H5. exact H0. exact H3.
+      * pose proof IHclos_trans_n1 l1 H2 st2 ((c0, Some l0, st0) :: stk) (eq_refl _).
+        repeat rewrite app_comm_cons in H0.
+        eapply middle_ceval'_while_loop, t_step in H0.
+        eapply t_trans.
+        exact H3. exact H0. exact H2.
+    + destruct stk; simpl in *; inversion H3; subst; clear H3.
+      destruct stk; simpl in *; inversion H7; subst; clear H7.
+      * pose proof IHclos_trans_n1 l1 H2 (loc1, glb) nil (eq_refl _).
+        rewrite <- (@app_nil_l (_ * _ * _)) in H0 at 1.
+        rewrite (cons_insert_nil (snd (fc f), Some (com_to_label_pure (snd (fc f))), (loc2, glb))), app_comm_cons in H0.
+        eapply middle_ceval'_while_loop, t_step in H0.
+        eapply t_trans.
+        exact H3. exact H0. exact H2.
+      * pose proof IHclos_trans_n1 l1 H2 st2 ((c1, Some l0, (loc1, glb)) :: stk) (eq_refl _).
+        repeat rewrite app_comm_cons in H0.
+        eapply middle_ceval'_while_loop, t_step in H0.
+        eapply t_trans.
+        exact H3. exact H0. exact H2.
+    + destruct stk; simpl in *; inversion H3; subst; clear H3.
+      * pose proof IHclos_trans_n1 l1 H2 (loc2, glb2) ((c1, None, (loc1, glb1)) :: nil) (eq_refl _).
+        rewrite <- app_nil_l in H0.
+        rewrite cons_insert_nil, app_comm_cons in H0.
+        eapply middle_ceval'_while_loop, t_step in H0.
+        eapply t_trans.
+        exact H3. exact H0. exact H2.
+      * pose proof IHclos_trans_n1 l1 H2 st2 ((c1, None, (loc1, glb1)) :: (c2, Some l2, (loc2, glb2)) :: stk) (eq_refl _).
+        repeat rewrite app_comm_cons in H0.
+        eapply middle_ceval'_while_loop, t_step in H0.
+        eapply t_trans.
+        exact H3. exact H0. exact H2.
+Qed.
+
+(* Lemma multi_ceval'_while_loop:
+  forall fc lf b c l1 st1 st2,
+  clos_trans restk (middle_ceval' fc lf)
+    ((c, Some l1, st1) :: nil)
+    ((c, None, st2) :: nil) ->
+  clos_trans restk (middle_ceval' fc lf)
+    ((CWhile b c, Some (LWhile b l1), st1) :: nil)
+    ((CWhile b c, Some (LWhile b (com_to_label_pure c)), st2) :: nil).
+Proof.
+  intros.
+  apply Operators_Properties.clos_trans_t1n in H.
+  set (stk := @nil (com * option label * state)).
+  unfold stk.
+  change ((c, Some l1, st1) :: nil) with (stk ++ (c, Some l1, st1) :: nil) in H.
+  change ((CWhile b c, Some (LWhile b l1), st1) :: nil) with (stk ++ (CWhile b c, Some (LWhile b l1), st1) :: nil).
+  clearbody stk.
+  remember (stk ++ (c, Some l1, st1) :: nil) as stk1.
+  remember ((c, None, st2) :: nil) as stk2.
+  generalize dependent stk.
+  revert st1.
+  generalize dependent l1.
+  induction H; intros; subst.
+  - destruct stk; simpl in *; inversion H; subst.
+    + pose proof ceval'_valid_label _ _ _ _ _ _ H3 as [? _].
+      destruct H0.
+(*       * eapply E'_WhileTrue2, ME_r_single in H3. admit. *)
+      * admit.
+      * admit.
+      + pose proof (eq_refl (length (stk ++ (c, Some l1, st1) :: nil))).
+      rewrite H7 in H0 at 1.
+      rewrite app_length in H0.
+      simpl in H0. omega.
+  - specialize (IHclos_trans_1n (eq_refl _)).
+    inversion H; subst.
+Admitted. *)
+(** While Loop *)
+
 Theorem ceval'_derive_multi_ceval_correct : ceval'_derive_multi_ceval.
 Proof.
   unfold ceval'_derive_multi_ceval.
@@ -981,16 +1374,116 @@ Proof.
         inversion H2; inversion H10; assumption.
       * pose proof com_to_label_pure_no_point c2.
         tauto.
-  - admit.
-  - admit.
-  - admit.
-  - admit.
+  - apply Operators_Properties.clos_trans_t1n in IHceval.
+    inversion IHceval; subst.
+    + inversion H1; subst.
+      apply t_step, ME_r_pure.
+      apply E'_IfTrue.
+      apply com_to_label_pure_is_pure.
+      apply com_to_label_pure_valid.
+      exact H.
+      exact H5.
+    + inversion H1; subst.
+      * inversion H2; inversion H3.
+      * apply Operators_Properties.clos_t1n_trans in H2.
+        epose proof multi_ceval'_if_branch _ _ _ _ _ _ _ _ H10 H2.
+        eapply E'_IfTrue, ME_r_single, t_step in H11.
+        eapply t_trans.
+        exact H11. apply H3.
+        apply SP_If1. exact H10.
+        apply com_to_label_pure_is_pure.
+        apply com_to_label_pure_is_pure.
+        right. exact H10.
+        exact H.
+      * pose proof com_to_label_pure_no_point c1.
+        congruence.
+  - apply Operators_Properties.clos_trans_t1n in IHceval.
+    inversion IHceval; subst.
+    + inversion H1; subst.
+      apply t_step, ME_r_pure.
+      apply E'_IfFalse.
+      apply com_to_label_pure_is_pure.
+      apply com_to_label_pure_valid.
+      exact H.
+      exact H5.
+    + inversion H1; subst.
+      * inversion H2; inversion H3.
+      * apply Operators_Properties.clos_t1n_trans in H2.
+        epose proof multi_ceval'_else_branch _ _ _ _ _ _ _ _ H10 H2.
+        eapply E'_IfFalse, ME_r_single, t_step in H11.
+        eapply t_trans; [apply H11 | apply H3].
+        apply SP_If2. apply com_to_label_pure_is_pure. exact H10.
+        apply com_to_label_pure_is_pure. right. exact H10.
+        assumption.
+      * pose proof com_to_label_pure_no_point c2.
+        congruence.
+  - apply t_step, ME_r_pure, E'_WhileFalse.
+    exact H.
+  - simpl in *.
+    apply Operators_Properties.clos_trans_tn1 in IHceval1.
+    apply Operators_Properties.clos_trans_t1n in IHceval2.
+    inversion IHceval1; inversion IHceval2; subst.
+    + inversion H2; inversion H4; subst.
+      epose proof E'_WhileTrue2 _ _ _ _ _ _ _ _ _ _ H H7 H15.
+      eapply ME_r_pure, t_step in H3.
+      exact H3.
+      Unshelve.
+      apply com_to_label_pure_valid.
+      apply com_to_label_pure_is_pure.
+      apply com_to_label_pure_is_pure.
+      apply com_to_label_pure_valid.
+      apply IP_While, com_to_label_pure_is_pure.
+      apply com_to_label_pure_valid.
+    + inversion H2; inversion H4; subst.
+      * epose proof E'_WhileTrue2 _ _ _ _ _ _ _ _ _ _ H H8 H20.
+        eapply ME_r_pure in H3.
+        pose proof t1n_trans _ _ _ _ _ H3 H5.
+        apply Operators_Properties.clos_t1n_trans in H6.
+        exact H6.
+        Unshelve.
+        apply IP_While, com_to_label_pure_is_pure.
+        left. apply com_to_label_pure_is_pure.
+      * epose proof E'_WhileTrue2 _ _ _ _ _ _ _ _ _ _ H H8 H21.
+        eapply ME_r_single in H3.
+        pose proof t1n_trans _ _ _ _ _ H3 H5.
+        apply Operators_Properties.clos_t1n_trans in H6.
+        exact H6.
+        Unshelve.
+        exact H20.
+        apply IP_While, com_to_label_pure_is_pure.
+        right; assumption.
+      * inversion H22.
+        pose proof com_to_label_pure_no_point c.
+        congruence.
+    + inversion H2; inversion H5; subst.
+      epose proof E'_WhileSeg2 _ _ _ _ _ _ _ _ _ _ H9 H15.
+      eapply ME_r_pure in H4.
+      apply Operators_Properties.clos_tn1_trans in H3.
+      eapply multi_ceval'_while_loop in H3.
+      eapply t_trans.
+      exact H3. apply t_step. exact H4.
+      assumption.
+    + inversion H2; inversion H5; subst.
+      * inversion H6; inversion H4.
+      * epose proof E'_WhileSeg2 _ _ _ _ _ _ _ _ _ _ H10 H21.
+        eapply ME_r_single, t_step in H4.
+        apply Operators_Properties.clos_tn1_trans in H3.
+        apply Operators_Properties.clos_t1n_trans in H6.
+        eapply t_trans.
+        2:{ exact H6. }
+        eapply t_trans.
+        2:{ exact H4. }
+        apply multi_ceval'_while_loop; try assumption.
+        exact H20.
+      * inversion H22.
+        pose proof com_to_label_pure_no_point c.
+        congruence.
   - admit.
 Unshelve.
+  inversion H3; inversion H4; assumption.
   left. apply com_to_label_pure_is_pure.
-  apply com_to_label_pure_is_pure.
-  apply com_to_label_pure_is_pure.
-  left. apply com_to_label_pure_is_pure.
+  inversion H3; inversion H4; assumption.
+  right; assumption.
 Admitted.
 (*   remember (snd (fc f)) as c.
   revert f Heqc.
